WIP

src/Specific/X86/Exponent25519.v
@@ -1,5 +1,6 @@
-Require Import Coq.ZArith.ZArith.
+Require Import Coq.ZArith.ZArith Coq.micromega.Psatz.
 Require Import Crypto.Spec.Ed25519.
+Require Import Crypto.Specific.X86.Core.
 Require Import Crypto.EdDSARepChange.
 Require Import Crypto.BoundedArithmetic.Interface.
 Require Import Crypto.BoundedArithmetic.X86ToZLike.
@@ -7,30 +8,188 @@ Require Import Crypto.BoundedArithmetic.X86ToZLikeProofs.
 Require Import Crypto.ModularArithmetic.BarrettReduction.ZBounded.
 Require Import Crypto.Util.Tuple.
 Require Import Crypto.Util.LetIn.
+Import NPeano.
 
-Local Notation modulus := (2^252 + 27742317777372353535851937790883648493)%Z.
+Local Notation modulusv := (2^252 + 27742317777372353535851937790883648493)%Z.
 Local Coercion Z.of_nat : nat >-> Z.
 Local Notation eta x := (fst x, snd x).
 Local Notation eta3 x := (eta (fst x), snd x).
 Local Notation eta4 x := (eta3 (fst x), snd x).
 Local Notation eta4' x := (eta (fst x), eta (snd x)).
 
-Section x86_64.
-  Local Notation n := 64%nat.
+Section x86.
   Local Notation base := 2%Z (* TODO(@andres-erbsen): Is this the correct base, or are we using something else? *).
   Local Notation smaller_bound_exp := 250%Z (* TODO(@andres-erbsen): Is this the correct smaller size (2^250), or are we using something else? *).
-  Context (ops : x86.instructions n) (props : x86.arithmetic ops).
-  Local Notation W := (tuple (tuple x86.W 2) 2) (* 256-bit words *).
-  Let ops' ldi_modulus ldi_0 : ZBounded.ZLikeOps (2^256) (2^smaller_bound_exp) modulus
-    := (@ZLikeOps_of_x86_64_Factored ops modulus smaller_bound_exp ldi_modulus ldi_0).
-  Local Existing Instance ops'.
-  Lemma modulus_in_range : (0 <= modulus < 2 ^ 256)%Z. Proof. vm_compute; intuition congruence. Qed.
   Lemma smaller_bound_smaller : (0 <= smaller_bound_exp <= 256)%Z. Proof. vm_compute; intuition congruence. Qed.
-  Lemma n_pos : (0 < 64%nat)%Z. Proof. vm_compute; intuition congruence. Qed.
+  Lemma modulusv_in_range : 0 <= modulusv < 2 ^ 256. Proof. vm_compute; intuition congruence. Qed.
+  Lemma modulusv_pos : 0 < modulusv. Proof. vm_compute; reflexivity. Qed.
+  Section gen_modulus.
+    Context (modulus : Z)
+            (modulus_in_range : 0 <= modulus < 2 ^ 256)
+            (modulus_pos : 0 < modulus).
+    Section gen.
+      Context (half_n : nat).
+      Local Notation n := (2 * half_n)%nat.
+      Context (ops : x86.instructions n) (props : x86.arithmetic ops)
+              (n_pos : (0 < n)%Z)
+              (n_pow_2 : (2^Nat.log2 (256 / n) = 256)%Z).
+      Let ops' ldi_modulus ldi_0 : ZBounded.ZLikeOps (2^256) (2^smaller_bound_exp) modulus
+        := (@ZLikeOps_of_x86_gen_Factored 256 n ops modulus smaller_bound_exp ldi_modulus ldi_0).
+      Local Existing Instance ops'.
+      Lemma full_width_pos : (0 < 256)%Z. Proof. omega. Qed.
+      Let props' ldi_modulus ldi_0 Hldi_modulus Hldi_0 : ZBounded.ZLikeProperties (ops' ldi_modulus ldi_0)
+        := @ZLikeProperties_of_x86_gen_Factored half_n 256 ops modulus props ldi_modulus ldi_0 Hldi_modulus Hldi_0 modulus_in_range smaller_bound_exp smaller_bound_smaller n_pos full_width_pos.
+      Local Existing Instance props'.
 
-  Let props' ldi_modulus ldi_0 Hldi_modulus Hldi_0 : ZBounded.ZLikeProperties (ops' ldi_modulus ldi_0)
-    := @ZLikeProperties_of_x86_64_Factored ops modulus props ldi_modulus ldi_0 Hldi_modulus Hldi_0 modulus_in_range smaller_bound_exp smaller_bound_smaller n_pos.
-  Local Existing Instance props'.
+      Let offset'0 := Eval compute in ((256 - smaller_bound_exp) / 2)%Z.
+      Let k'0 := Eval compute in ((256 - offset'0) / Z.log2 base)%Z.
+      Section params_gen.
+        Import BarrettBundled.
+        Context (ldi_modulus ldi_0 ldi_μ0 : Core.repeated_tuple x86.W 2 (Nat.log2 (256 / n))).
+        Let offset' := Eval compute in offset'0.
+        Let k' := Eval compute in k'0.
+        Local Instance x86_25519_Barrett : BarrettParameters
+          := { m := modulus;
+               b := base;
+               k := k';
+               offset := offset';
+               ops := ops' ldi_modulus ldi_0;
+               μ' := ldi_μ0 }.
+        Local Instance x86_25519_BarrettProofs
+              Hldi_modulus Hldi_0
+              (Hldi_μ0 : ldi_μ0 = ldi μ)
+              (H0 : 3 * m <= b ^ (k + offset))
+              (H1 : b ^ (k - offset) <= m + 1)
+              (H2 : (0 <= μ < 2 ^ (256 * n)))
+          : BarrettParametersCorrect x86_25519_Barrett
+          := { props := props' ldi_modulus ldi_0 Hldi_modulus Hldi_0 }.
+        Proof.
+          assumption.
+          vm_compute; reflexivity.
+          vm_compute; clear; abstract intuition congruence.
+          vm_compute; clear; abstract intuition congruence.
+          assumption.
+          assumption.
+          vm_compute; exact I.
+          { cbv [μ μ' x86_25519_Barrett ZBounded.decode_small BarrettBundled.ops ops' ZLikeOps_of_x86_64 ZLikeOps_of_x86_64_Factored ZLikeOps_of_x86_gen_Factored ZBounded.SmallT b k m offset].
+            clear -props Hldi_μ0 n_pow_2 n_pos H2.
+            abstract (
+                subst ldi_μ0;
+                assert (2^256 <= 2^(256 * n)) by (clear -n_pos; auto with zarith omega);
+                rewrite decode_load_immediate
+                  by solve [ exact _ | change (Z.of_nat 2) with 2%Z; rewrite n_pow_2; exact H2 ];
+                reflexivity
+              ). }
+        Defined.
+      End params_gen.
+      Local Existing Instance x86_25519_Barrett.
+      Local Existing Instance x86_25519_BarrettProofs.
+      Definition ldi_modulus : Core.repeated_tuple x86.W 2 (Nat.log2 (256 / n)) := ldi modulus.
+      Definition ldi_mod_inverse : Core.repeated_tuple x86.W 2 (Nat.log2 (256 / n)) := ldi (base^(2*k'0) / modulus).
+      Definition barrett_reduce (x : tuple (Core.repeated_tuple x86.W 2 (Nat.log2 (256 / n))) 2)
+        : Core.repeated_tuple x86.W 2 (Nat.log2 (256 / n))
+        := dlet ldi_modulus' := ldi_modulus in
+           dlet ldi_μ := ldi_mod_inverse in
+           dlet ldi_0 := ldi 0 in
+           let params := x86_25519_Barrett ldi_modulus' ldi_0 ldi_μ in
+           barrett_reduce_function_bundled x.
+    End gen.
+
+    Section x86_64.
+      Local Notation n := 64%nat.
+      Context (ops : x86.instructions n) (props : x86.arithmetic ops).
+      Lemma n64_pos : (0 < n)%Z. Proof. vm_compute; intuition congruence. Qed.
+      Local Notation W := (tuple (tuple x86.W 2) 2) (* 256-bit words *).
+      Local Arguments barrett_reduce / _ _ _ .
+      Local Arguments Core.load_immediate_double / _ _ _ _.
+      Local Arguments Z.modulo !_ !_ / .
+      Local Arguments Z.pow_pos !_ !_ / .
+      Local Arguments Z.div !_ !_ / .
+      Local Arguments barrett_reduce_function_bundled : simpl never.
+      Local Opaque Let_In ldi_mod_inverse ldi_modulus.
+      Definition barrett_reduce64'0 (x : tuple W 2) : W
+        := Eval simpl in @barrett_reduce 32 ops x.
+      Definition barrett_reduce64'1 (x : tuple W 2) : W
+        := Eval cbv [barrett_reduce64'0 tuple barrett_reduce_function_bundled barrett_reduce_function
+                                        BarrettBundled.m BarrettBundled.b BarrettBundled.k BarrettBundled.offset BarrettBundled.μ' x86_25519_Barrett
+                                        ZBounded.ConditionalSubtractModulus ZBounded.CarrySubSmall ZBounded.Mod_SmallBound ZBounded.Mod_SmallBound ZBounded.Mul ZBounded.DivBy_SmallBound ZBounded.DivBy_SmallerBound ZBounded.modulus_digits ZBounded.SmallT ZBounded.LargeT BarrettBundled.ops ZLikeOps_of_x86_gen_Factored]
+          in @barrett_reduce64'0 x.
+      Local Opaque Core.sub_with_carry_repeated_double Core.multiply_double_repeated_double
+            Core.shift_right_doubleword_immediate_repeated_double
+            Core.select_conditional_repeated_double.
+      Local Arguments barrett_reduce64'1 / _.
+      Definition barrett_reduce64'2 (x : tuple W 2) : W
+        := Eval simpl in @barrett_reduce64'1 x.
+      Local Transparent Core.sub_with_carry_repeated_double Core.multiply_double_repeated_double
+            Core.shift_right_doubleword_immediate_repeated_double
+            Core.select_conditional_repeated_double.
+      Definition barrett_reduce64'3 (x : tuple W 2) : W
+        := Eval cbv [barrett_reduce64'2
+                       tuple Core.repeated_tuple tuple'
+                       fst snd (*Interface.ldi Interface.muldw Interface.mulhwll Interface.mulhwhl Interface.mulhwhh Interface.shl Interface.shr Interface.or Interface.shrd Interface.adc Interface.subc Interface.selc Interface.adc Interface.subc*)
+                       Core.select_conditional_repeated_double Core.selc_double Core.select_conditional_double
+                       Core.multiply_double_repeated_double Core.mul_double_multiply Core.mul_double Core.mul_double_multiply_low_low Core.mul_double_multiply_high_low Core.mul_double_multiply_high_high
+                       Core.shift_right_doubleword_immediate_repeated_double Core.shift_right_doubleword_immediate_double Core.shrd_double
+                       Core.shlr_repeated_double
+                       Core.shift_right_immediate_repeated_double Core.shift_left_immediate_repeated_double
+                       Core.shift_left_immediate_double Core.shift_right_immediate_double
+                       Core.shr_double Core.shl_double
+                       Core.load_immediate_repeated_double Core.ldi_double Core.load_immediate_double
+                       Core.ripple_carry_adc Core.ripple_carry_subc
+                       Core.sub_with_carry_repeated_double Core.add_with_carry_repeated_double
+                       Core.ripple_carry_tuple
+                       Core.ripple_carry_tuple'
+                       StripCF.shift_left_immediate_strip_CF StripCF.shift_right_immediate_strip_CF StripCF.bitwise_or_strip_CF StripCF.shift_right_doubleword_immediate_strip_CF StripCF.multiply_double_strip_CF
+                       Nat.log2 Nat.div Nat.divmod Nat.pred Nat.log2_iter Core.ripple_carry_subc Z.of_nat Pos.of_succ_nat Z.pow Z.mul Z.eqb Z_eq_bool Pos.eqb Z.sub Z.ltb Z.leb Z.gtb Z.geb Pos.sub Pos.ltb Pos.leb Z.opp Z.add Pos.add Z.compare Z.pos_sub  Pos.compare Pos.compare_cont Z.pow_pos Pos.succ Pos.mul Pos.iter Z.succ_double Z.double Pos.pred_double
+                       Z.modulo Z.div Z.div_eucl Z.pos_div_eucl Z.ltb Z.leb Pos.ltb Pos.leb Pos.compare Pos.compare_cont Z.compare fst snd Z.mul Pos.mul Z.add Pos.add Z.sub Z.opp Z.pos_sub Z.double Z.succ_double Pos.pred_double Z.pred_double]
+          in @barrett_reduce64'2 x.
+      Local Arguments barrett_reduce64'3 / _ .
+    End x86_64.
+  End gen_modulus.
+
+  Section x86_64.
+    Local Notation n := 64%nat.
+      Context (ops : x86.instructions n) (props : x86.arithmetic ops).
+      Local Notation W := (tuple (tuple x86.W 2) 2) (* 256-bit words *).
+
+      Definition barrett_reduce64'4 (x : tuple W 2) : W.
+      Proof.
+        let ldiμ := constr:(ldi_mod_inverse modulusv 32 ops) in
+        let ldiμv := (eval cbv [ldi_mod_inverse Core.load_immediate_repeated_double Core.ldi_double Core.load_immediate_double Nat.mul Nat.add Nat.div fst PeanoNat.Nat.divmod Nat.log2 Nat.log2_iter Nat.pred Core.repeated_tuple tuple tuple'] in ldiμ) in
+        let arg := constr:(@Interface.ldi x86.W x86.ldi) in
+        let ldiμv := match (eval pattern arg in ldiμv) with ?P _ => P end in
+        let ldiμv := (eval vm_compute in ldiμv) in
+        let ldiμv := (eval cbv beta in (ldiμv arg)) in
+        let ldimodulus := constr:(ldi_modulus modulusv 32 ops) in
+        let ldimodulusv := (eval cbv [ldi_modulus Core.load_immediate_repeated_double Core.ldi_double Core.load_immediate_double Nat.mul Nat.add Nat.div fst PeanoNat.Nat.divmod Nat.log2 Nat.log2_iter Nat.pred Core.repeated_tuple tuple tuple'] in ldimodulus) in
+        let arg := constr:(@Interface.ldi x86.W x86.ldi) in
+        let ldimodulusv := match (eval pattern arg in ldimodulusv) with ?P _ => P end in
+        let ldimodulusv := (eval vm_compute in ldimodulusv) in
+        let ldimodulusv := (eval cbv beta in (ldimodulusv arg)) in
+        let v := constr:(@barrett_reduce64'3 modulusv ops x) in
+        let v := (eval cbv beta iota delta [barrett_reduce64'3] in v) in
+        let v := match v with
+                 | appcontext v'[ldiμ]
+                   => let v := context v'[ldiμv] in
+                      v
+                 end in
+        let v := match v with
+                 | appcontext v'[ldimodulus]
+                   => let v := context v'[ldimodulusv] in
+                      v
+                 end in
+        pose v.
+        ldi_modulus modulusv 32 ops
+        let
+          := Eval simpl in @barrett_reduce64'3 x.
+      Print barrett_reduce64.
+
+
+      Eval cbv [ barrett_reduce64'3  fst snd    ] in barrett_reduce64'3.
+
+      StripCF.multiply_double_strip_CF
+      Lemma modulus_in_range : (0 <= modulus < 2 ^ 256)%Z. Proof. vm_compute; intuition congruence. Qed.
+
 
   Section params_64.
     Import BarrettBundled.
