src/Specific/X86/Core.v
@@ -1,0 +1,281 @@
+(** * An x86 Machine *)
+Require Import Coq.Classes.RelationClasses Coq.Classes.Morphisms.
+Require Import Coq.PArith.BinPos Coq.micromega.Psatz.
+Require Export Coq.ZArith.ZArith Coq.Lists.List.
+Require Import Crypto.Util.Decidable.
+Require Export Crypto.BoundedArithmetic.Interface.
+Require Export Crypto.BoundedArithmetic.ArchitectureToZLike.
+Require Export Crypto.BoundedArithmetic.ArchitectureToZLikeProofs.
+Require Export Crypto.Util.Tuple.
+Require Import Crypto.Util.Option Crypto.Util.Sigma Crypto.Util.Prod.
+Require Export Crypto.Reflection.Named.Syntax.
+Require Import Crypto.Reflection.Named.DeadCodeElimination.
+Require Import Crypto.Reflection.CountLets.
+Require Import Crypto.Reflection.Named.ContextOn.
+Require Export Crypto.Reflection.Syntax.
+Require Import Crypto.Reflection.Linearize.
+Require Import Crypto.Reflection.Inline.
+Require Import Crypto.Reflection.CommonSubexpressionElimination.
+Require Export Crypto.Reflection.Reify.
+Require Export Crypto.Util.ZUtil.
+Require Export Crypto.Util.Notations.
+Require Import Crypto.Util.ListUtil.
+Require Export Crypto.Util.LetIn.
+Export ListNotations.
+
+Open Scope Z_scope.
+Local Notation eta x := (fst x, snd x).
+Local Notation eta3 x := (eta (fst x), snd x).
+Local Notation eta3' x := (fst x, eta (snd x)).
+
+(** ** Reflective Assembly Syntax *)
+Section reflection.
+  Context {n} (ops : x86.instructions n).
+  Local Set Boolean Equality Schemes.
+  Local Set Decidable Equality Schemes.
+  Inductive base_type := TZ | Tbool | TW.
+  Global Instance dec_base_type : DecidableRel (@eq base_type)
+    := base_type_eq_dec.
+  Definition interp_base_type (v : base_type) : Type :=
+    match v with
+    | TZ => Z
+    | Tbool => bool
+    | TW => x86.W
+    end.
+  Local Notation tZ := (Tbase TZ).
+  Local Notation tbool := (Tbase Tbool).
+  Local Notation tW := (Tbase TW).
+  Local Open Scope ctype_scope.
+  Print x86.instructions.
+  Inductive op : flat_type base_type -> flat_type base_type -> Type :=
+  | OPldi     : op tZ tW
+  | OPshrd    : op (tW * tW * tZ) (tbool * tW)
+  | OPshl     : op (tW * tZ) (tbool * tW)
+  | OPshr     : op (tW * tZ) (tbool * tW)
+  | OPadc     : op (tW * tW * tbool) (tbool * tW)
+  | OPsubc    : op (tW * tW * tbool) (tbool * tW)
+  | OPmuldw   : op (tW * tW) (tbool * (tW * tW))
+  | OPselc    : op (tbool * tW * tW) tW
+  | OPor      : op (tW * tW) (tbool * tW).
+
+  Definition interp_op src dst (f : op src dst)
+    : interp_flat_type_gen interp_base_type src -> interp_flat_type_gen interp_base_type dst
+    := match f in op s d return interp_flat_type_gen _ s -> interp_flat_type_gen _ d with
+       | OPldi     => ldi
+       | OPshrd    => fun xyz => let '(x, y, z) := eta3 xyz in shrdf x y z
+       | OPshl     => fun xy => let '(x, y) := eta xy in shlf x y
+       | OPshr     => fun xy => let '(x, y) := eta xy in shrf x y
+       | OPadc     => fun xyz => let '(x, y, z) := eta3 xyz in adc x y z
+       | OPsubc    => fun xyz => let '(x, y, z) := eta3 xyz in subc x y z
+       | OPmuldw   => fun xy => let '(x, y) := eta xy in muldwf x y
+       | OPselc    => fun xyz => let '(x, y, z) := eta3 xyz in selc x y z
+       | OPor      => fun xy => let '(x, y) := eta xy in orf x y
+       end.
+
+  Definition Inline {t} e := @InlineConst base_type interp_base_type op t e.
+End reflection.
+
+Ltac base_reify_op op op_head ::=
+     lazymatch op_head with
+     | @Interface.ldi => constr:(reify_op op op_head 1 OPldi)
+     | @Interface.shrdf => constr:(reify_op op op_head 3 OPshrd)
+     | @Interface.shlf => constr:(reify_op op op_head 2 OPshl)
+     | @Interface.shrf => constr:(reify_op op op_head 2 OPshr)
+     | @Interface.adc => constr:(reify_op op op_head 3 OPadc)
+     | @Interface.subc => constr:(reify_op op op_head 3 OPsubc)
+     | @Interface.muldwf => constr:(reify_op op op_head 2 OPmuldw)
+     | @Interface.selc => constr:(reify_op op op_head 3 OPselc)
+     | @Interface.orf => constr:(reify_op op op_head 3 OPor)
+     end.
+Ltac base_reify_type T ::=
+     match T with
+     | Z => TZ
+     | bool => Tbool
+     | x86.W => TW
+     end.
+
+Ltac Reify' e := Reify.Reify' base_type (interp_base_type _) op e.
+Ltac Reify e :=
+  let v := Reify.Reify base_type (interp_base_type _) op e in
+  constr:(Inline _ ((*CSE _*) (InlineConst (Linearize v)))).
+(*Ltac Reify_rhs := Reify.Reify_rhs base_type (interp_base_type _) op (interp_op _).*)
+
+(*
+(** ** Raw Syntax Trees *)
+(** These are used solely for pretty-printing the expression tree in a
+    form that can be basically copy-pasted into other languages which
+    can be compiled for the Fancy Machine.  Hypothetically, we could
+    add support for custom named identifiers, by carrying around
+    [string] identifiers and using them for pretty-printing...  It
+    might also be possible to verify this layer, too, by adding a
+    partial interpretation function... *)
+
+Local Set Decidable Equality Schemes.
+Local Set Boolean Equality Schemes.
+
+Inductive Register :=
+| RegPInv | RegMod | RegMuLow | RegZero
+| y | t1 | t2 | lo | hi | out | src1 | src2 | tmp | q | qHigh | x | xHigh
+| SpecialCarryBit
+| scratch | scratchplus (n : nat).
+
+Notation "'scratch+' n" := (scratchplus n) (format "'scratch+' n", at level 10).
+
+Definition pos_of_Register (r : Register) :=
+  match r with
+  | RegPInv => 1
+  | RegMod => 2
+  | RegMuLow => 3
+  | RegZero => 4
+  | y => 5
+  | t1 => 6
+  | t2 => 7
+  | lo => 8
+  | hi => 9
+  | out => 10
+  | src1 => 11
+  | src2 => 12
+  | tmp => 13
+  | q => 14
+  | qHigh => 15
+  | x => 16
+  | xHigh => 17
+  | SpecialCarryBit => 18
+  | scratch => 19
+  | scratchplus n => 19 + Pos.of_nat (S n)
+  end%positive.
+
+Lemma pos_of_Register_inj x y : pos_of_Register x = pos_of_Register y -> x = y.
+Proof.
+  unfold pos_of_Register; repeat break_match; subst;
+    try rewrite Pos.add_cancel_l; try rewrite Nat2Pos.inj_iff;
+      try solve [ simpl; congruence | intros; exfalso; lia ].
+Qed.
+
+Global Instance RegisterContext {var : base_type -> Type} : Context Register var
+  := ContextOn pos_of_Register (RegisterAssign.pos_context var).
+
+Definition syntax {ops : fancy_machine.instructions (2 * 128)}
+  := Named.expr base_type (interp_base_type ops) op Register.
+
+Class wf_empty {ops} {var} {t} (e : Named.expr base_type (interp_base_type ops) op Register t)
+  := mk_wf_empty : @Named.wf base_type (interp_base_type ops) op Register var _ empty t e.
+Global Hint Extern 0 (wf_empty _) => vm_compute; intros; constructor : typeclass_instances.
+
+(** Assemble a well-typed easily interpretable expression into a
+    syntax tree we can use for pretty-printing. *)
+Section assemble.
+  Context {ops : fancy_machine.instructions (2 * 128)}.
+
+  Definition AssembleSyntax' {t} (e : Expr base_type (interp_base_type _) op t) (ls : list Register)
+    : option (syntax t)
+    := CompileAndEliminateDeadCode e ls.
+  Definition AssembleSyntax {t} e ls (res := @AssembleSyntax' t e ls)
+    := match res return match res with None => _ | _ => _ end with
+       | Some v => v
+       | None => I
+       end.
+
+  Definition dummy_registers (n : nat) : list Register
+    := List.map scratchplus (seq 0 n).
+  Definition DefaultRegisters {t} (e : Expr base_type (interp_base_type _) op t) : list Register
+    := dummy_registers (CountBinders e).
+
+  Definition DefaultAssembleSyntax {t} e := @AssembleSyntax t e (DefaultRegisters e).
+
+  Definition Interp {t} e {wf : wf_empty e}
+    := @Named.interp base_type (interp_base_type _) op Register _ (interp_op _) empty t e wf.
+End assemble.
+
+Export Reflection.Named.Syntax.
+Open Scope nexpr_scope.
+Open Scope ctype_scope.
+Open Scope type_scope.
+Open Scope core_scope.
+
+Notation Return x := (Var x).
+Notation ldi z := (Op OPldi (Const z%Z)).
+Notation "'slet' x := A 'in' b" := (LetIn _ x (Op OPldi (Var A%nexpr)) b%nexpr) : nexpr_scope.
+Notation "'c.Rshi' ( x , A , B , C ) , b" :=
+  (LetIn _ x (Op OPshrd (Pair (Pair (Var A) (Var B)) (Const C%Z))) b)
+    (at level 200, b at level 200, format "'c.Rshi' ( x ,  A ,  B ,  C ) , '//' b").
+Notation "'c.Mul128' ( x , 'c.UpperHalf' ( A ) , 'c.UpperHalf' ( B ) ) , b" :=
+  (LetIn _ x (Op OPmulhwhh (Pair (Var A) (Var B))) b)
+    (at level 200, b at level 200, format "'c.Mul128' ( x ,  'c.UpperHalf' ( A ) ,  'c.UpperHalf' ( B ) ) , '//' b").
+Notation "'c.Mul128' ( x , 'c.UpperHalf' ( A ) , 'c.LowerHalf' ( B ) ) , b" :=
+  (LetIn _ x (Op OPmulhwhl (Pair (Var A) (Var B))) b)
+    (at level 200, b at level 200, format "'c.Mul128' ( x ,  'c.UpperHalf' ( A ) ,  'c.LowerHalf' ( B ) ) , '//' b").
+Notation "'c.Mul128' ( x , 'c.LowerHalf' ( A ) , 'c.LowerHalf' ( B ) ) , b" :=
+  (LetIn _ x (Op OPmulhwll (Pair (Var A) (Var B))) b)
+    (at level 200, b at level 200, format "'c.Mul128' ( x ,  'c.LowerHalf' ( A ) ,  'c.LowerHalf' ( B ) ) , '//' b").
+Notation "'c.LeftShifted' { x , v }" :=
+  (Op OPshl (Pair (Var x) (Const v%Z)))
+    (at level 200, format "'c.LeftShifted' { x ,  v }").
+Notation "'c.RightShifted' { x , v }" :=
+  (Op OPshr (Pair (Var x) (Const v%Z)))
+    (at level 200, format "'c.RightShifted' { x ,  v }").
+
+Notation "'c.Add' ( x , A , B ) , b" :=
+  (LetIn _ (pair SpecialCarryBit x) (Op OPadc (Pair (Pair A B) (Const false))) b)
+    (at level 200, b at level 200, format "'c.Add' ( x ,  A ,  B ) , '//' b").
+Notation "'c.Add' ( x , A , B ) , b" :=
+  (LetIn _ (pair SpecialCarryBit x) (Op OPadc (Pair (Pair (Var A) B) (Const false))) b)
+    (at level 200, b at level 200, format "'c.Add' ( x ,  A ,  B ) , '//' b").
+Notation "'c.Add' ( x , A , B ) , b" :=
+  (LetIn _ (pair SpecialCarryBit x) (Op OPadc (Pair (Pair A (Var B)) (Const false))) b)
+    (at level 200, b at level 200, format "'c.Add' ( x ,  A ,  B ) , '//' b").
+Notation "'c.Add' ( x , A , B ) , b" :=
+  (LetIn _ (pair SpecialCarryBit x) (Op OPadc (Pair (Pair (Var A) (Var B)) (Const false))) b)
+    (at level 200, b at level 200, format "'c.Add' ( x ,  A ,  B ) , '//' b").
+Notation "'c.Addc' ( x , A , B ) , b" :=
+  (LetIn _ (pair SpecialCarryBit x) (Op OPadc (Pair (Pair A B) (Var SpecialCarryBit))) b)
+    (at level 200, b at level 200, format "'c.Addc' ( x ,  A ,  B ) , '//' b").
+Notation "'c.Addc' ( x , A , B ) , b" :=
+  (LetIn _ (pair SpecialCarryBit x) (Op OPadc (Pair (Pair (Var A) B) (Var SpecialCarryBit))) b)
+    (at level 200, b at level 200, format "'c.Addc' ( x ,  A ,  B ) , '//' b").
+Notation "'c.Addc' ( x , A , B ) , b" :=
+  (LetIn _ (pair SpecialCarryBit x) (Op OPadc (Pair (Pair A (Var B)) (Var SpecialCarryBit))) b)
+    (at level 200, b at level 200, format "'c.Addc' ( x ,  A ,  B ) , '//' b").
+Notation "'c.Addc' ( x , A , B ) , b" :=
+  (LetIn _ (pair SpecialCarryBit x) (Op OPadc (Pair (Pair (Var A) (Var B)) (Var SpecialCarryBit))) b)
+    (at level 200, b at level 200, format "'c.Addc' ( x ,  A ,  B ) , '//' b").
+
+Notation "'c.Sub' ( x , A , B ) , b" :=
+  (LetIn _ (pair SpecialCarryBit x) (Op OPsubc (Pair (Pair A B) (Const false))) b)
+    (at level 200, b at level 200, format "'c.Sub' ( x ,  A ,  B ) , '//' b").
+Notation "'c.Sub' ( x , A , B ) , b" :=
+  (LetIn _ (pair SpecialCarryBit x) (Op OPsubc (Pair (Pair (Var A) B) (Const false))) b)
+    (at level 200, b at level 200, format "'c.Sub' ( x ,  A ,  B ) , '//' b").
+Notation "'c.Sub' ( x , A , B ) , b" :=
+  (LetIn _ (pair SpecialCarryBit x) (Op OPsubc (Pair (Pair A (Var B)) (Const false))) b)
+    (at level 200, b at level 200, format "'c.Sub' ( x ,  A ,  B ) , '//' b").
+Notation "'c.Sub' ( x , A , B ) , b" :=
+  (LetIn _ (pair SpecialCarryBit x) (Op OPsubc (Pair (Pair (Var A) (Var B)) (Const false))) b)
+    (at level 200, b at level 200, format "'c.Sub' ( x ,  A ,  B ) , '//' b").
+
+Notation "'c.Addm' ( x , A , B ) , b" :=
+  (LetIn _ x (Op OPaddm (Pair (Pair A B) (Var RegMod))) b)
+    (at level 200, b at level 200, format "'c.Addm' ( x ,  A ,  B ) , '//' b").
+Notation "'c.Addm' ( x , A , B ) , b" :=
+  (LetIn _ x (Op OPaddm (Pair (Pair (Var A) B) (Var RegMod))) b)
+    (at level 200, b at level 200, format "'c.Addm' ( x ,  A ,  B ) , '//' b").
+Notation "'c.Addm' ( x , A , B ) , b" :=
+  (LetIn _ x (Op OPaddm (Pair (Pair A (Var B)) (Var RegMod))) b)
+    (at level 200, b at level 200, format "'c.Addm' ( x ,  A ,  B ) , '//' b").
+Notation "'c.Addm' ( x , A , B ) , b" :=
+  (LetIn _ x (Op OPaddm (Pair (Pair (Var A) (Var B)) (Var RegMod))) b)
+    (at level 200, b at level 200, format "'c.Addm' ( x ,  A ,  B ) , '//' b").
+
+Notation "'c.Selc' ( x , A , B ) , b" :=
+  (LetIn _ x (Op OPselc (Pair (Pair (Var SpecialCarryBit) A) B)) b)
+    (at level 200, b at level 200, format "'c.Selc' ( x ,  A ,  B ) , '//' b").
+Notation "'c.Selc' ( x , A , B ) , b" :=
+  (LetIn _ x (Op OPselc (Pair (Pair (Var SpecialCarryBit) (Var A)) B)) b)
+    (at level 200, b at level 200, format "'c.Selc' ( x ,  A ,  B ) , '//' b").
+Notation "'c.Selc' ( x , A , B ) , b" :=
+  (LetIn _ x (Op OPselc (Pair (Pair (Var SpecialCarryBit) A) (Var B))) b)
+    (at level 200, b at level 200, format "'c.Selc' ( x ,  A ,  B ) , '//' b").
+Notation "'c.Selc' ( x , A , B ) , b" :=
+  (LetIn _ x (Op OPselc (Pair (Pair (Var SpecialCarryBit) (Var A)) (Var B))) b)
+    (at level 200, b at level 200, format "'c.Selc' ( x ,  A ,  B ) , '//' b").
+*)
